ll

examples/layeredeffects/LL.fst
@@ -4,22 +4,19 @@ module LL
 type epre_t = Type0
 type epost_t (a:Type) = option a -> Type0
 type ewp_t (a:Type) =
-  wp:(epost_t a -> epre_t)
-
-assume WP_m1 :
-  forall (a:Type) (wp:ewp_t a).
-    (forall p q.
-       (forall r. p r ==> q r) ==>
-       (wp p ==> wp q))
-       
+  wp:(epost_t a -> epre_t){
+    forall p q.
+      (forall r. p r ==> q r) ==>
+      (wp p ==> wp q)}
 
 type erepr (a:Type) (wp:ewp_t a) = unit -> PURE (option a) wp
 
-
+inline_for_extraction
 let ereturn (a:Type) (x:a)
 : erepr a (fun p -> p (Some x))
 = fun _ -> Some x
 
+inline_for_extraction
 let ebind (a:Type) (b:Type)
   (wp_f:ewp_t a) (wp_g:a -> ewp_t b)
   (f:erepr a wp_f) (g:(x:a -> erepr b (wp_g x)))
@@ -35,6 +32,7 @@ let ebind (a:Type) (b:Type)
   | None -> None
   | Some x -> g x ()
 
+inline_for_extraction
 let estronger (a:Type)
   (wp_f:ewp_t a) (wp_g:ewp_t a)
   (f:erepr a wp_f)
@@ -43,6 +41,7 @@ let estronger (a:Type)
   (ensures fun _ -> True)
 = f
 
+inline_for_extraction
 let econjunction (a:Type)
   (wp_f:ewp_t a) (wp_g:ewp_t a)
   (f:erepr a wp_f) (g:erepr a wp_g)
@@ -53,7 +52,7 @@ let econjunction (a:Type)
     (p ==> wp_f post) /\
     ((~ p) ==> wp_g post))
 
-
+reifiable reflectable
 layered_effect {
   EXN : a:Type -> ewp_t a -> Effect
   with
@@ -64,18 +63,15 @@ layered_effect {
   conjunction = econjunction
 }
 
-
-assume WP_m2 :
-  forall (a:Type) (wp:pure_wp a).
-    (forall p q.
-       (forall x. p x ==> q x) ==>
-       (wp p ==> wp q))
-
-let lift_pure_exn (a:Type) (wp:pure_wp a) (f:unit -> PURE a wp)
+inline_for_extraction
+let lift_pure_exn (a:Type) (wp:pure_wp a{forall p q. (forall x. p x ==> q x) ==> (wp p ==> wp q)}) (f:unit -> PURE a wp)
 : erepr a (fun p -> wp (fun x -> p (Some x)))
 = fun _ -> Some (f ())
 
 sub_effect PURE ~> EXN = lift_pure_exn
+
+effect Exn (a:Type) (pre:Type0) (post:option a -> Type0) =
+  EXN a (fun p -> pre /\ (forall r. post r ==> p r))
 
 
 
@@ -90,61 +86,227 @@ let monotonic_wp (#a:Type) (wp:wp_t0 a) =
     (forall n. wp p n ==> wp q n)
 
 type wp_t (a:Type) =
-  wp:(post_t a -> pre_t){monotonic_wp wp}
+  wp:wp_t0 a{monotonic_wp wp}
 
 type repr (a:Type) (wp:wp_t a) =
   n:nat -> EXN (a & nat) (fun p -> wp p n)
 
+inline_for_extraction
 let return (a:Type) (x:a)
 : repr a (fun p n -> p (Some (x, n)))
 = fun n -> (x, n)
 
-#set-options "--max_fuel 0 --initial_ifuel 4 --max_ifuel 4"
+//#set-options "--max_fuel 0 --initial_ifuel 4 --max_ifuel 4"
 
-let lemma_monotonic (#a:Type) (wp:wp_t a) (p:post_t a) (q:post_t a) (n:nat)
-: Lemma
-  (requires forall r. p r ==> q r)
-  (ensures wp p n ==> wp q n)
-= ()
-
+unfold
 let post_a (a:Type) (b:Type) (wp_g:a -> wp_t b) (p:post_t b) : post_t a =
   fun r ->
   match r with
   | None -> p None
   | Some r -> Prims.auto_squash (wp_g (Mktuple2?._1 r) p (Mktuple2?._2 r))
 
+let lemma_monotonic2 (#a:Type) (#b:Type) (wp_f:wp_t a) (wp_g:a -> wp_t b) (p:post_t b) (q:post_t b) (n:nat)
+: Lemma
+  (requires forall (r:option (a & nat)). post_a a b wp_g p r ==> post_a a b wp_g q r)
+  (ensures wp_f (post_a a b wp_g p) n ==> wp_f (post_a a b wp_g q) n)
+= admit ()
+
 unfold
 let bind_wp0 (a:Type) (b:Type) (wp_f:wp_t a) (wp_g:a -> wp_t b) : post_t b -> pre_t =
   fun p n -> wp_f (post_a a b wp_g p) n
 
-//#restart-solver
-//#set-options "--log_queries"
-
 open FStar.Tactics
 
-#set-options "--print_full_names --print_implicits --print_bound_var_types" //--debug_level Rel --debug LL"
+unfold
 let bind_wp (a:Type) (b:Type) (wp_f:wp_t a) (wp_g:a -> wp_t b) : wp_t b
 = assert (monotonic_wp (bind_wp0 a b wp_f wp_g)) by
-    (//compute ();
-     //ignore (forall_intro ());
-     //ignore (forall_intro ());
-     //ignore (implies_intro ());
-     //ignore (forall_intro ());
-     //apply_lemma (`lemma_monotonic);
-     norm [delta_only [`%monotonic_wp]];
-     ignore (forall_intro ());
-     ignore (forall_intro ());
+    (norm [delta_only [`%monotonic_wp]];
+     let p_binder = forall_intro () in
+     let q_binder = forall_intro () in
      ignore (implies_intro ());
      ignore (forall_intro ());
      norm [delta_only [`%bind_wp0]];
-     apply_lemma (`lemma_monotonic);
-     dump "C");
+     let wp_f_binder, wp_g_binder =
+       match (cur_binders ()) with
+       | _::_::wp_f::wp_g::_ -> wp_f, wp_g
+       | _ -> fail "" in
+     apply_lemma (`(lemma_monotonic2 (`#(binder_to_term wp_f_binder)) (`#(binder_to_term wp_g_binder)) (`#(binder_to_term p_binder)) (`#(binder_to_term q_binder))));
+     norm [delta_only [`%post_a]];
+     ignore (forall_intro ()));
   bind_wp0 a b wp_f wp_g
 
-// let bind (a:Type) (b:Type)
-//   (wp_f:wp_t a) (wp_g:a -> wp_t b)
-//   (f:repr a wp_f) (g:(x:a -> repr b (wp_g x)))
-// : repr b (bind_wp a b wp_f wp_g)
-// = fun n ->
-//   let (x, n) = f n in
-//   g x n
+inline_for_extraction
+let bind (a:Type) (b:Type)
+  (wp_f:wp_t a) (wp_g:a -> wp_t b)
+  (f:repr a wp_f) (g:(x:a -> repr b (wp_g x)))
+: repr b (bind_wp a b wp_f wp_g)
+= fun n ->
+  let (x, n) = f n in
+  g x n
+
+inline_for_extraction
+let stronger (a:Type)
+  (wp_f:wp_t a) (wp_g:wp_t a)
+  (f:repr a wp_f)
+: Pure (repr a wp_g)
+  (requires forall p n. wp_g p n ==> wp_f p n)
+  (ensures fun _ -> True)
+= f
+
+inline_for_extraction
+let conjunction (a:Type)
+  (wp_f:wp_t a) (wp_g:wp_t a)
+  (f:repr a wp_f) (g:repr a wp_g)
+  (p:Type0)
+: Type
+= repr a
+  (fun post n ->
+    (p ==> wp_f post n) /\
+    ((~ p) ==> wp_g post n))
+
+reifiable reflectable
+layered_effect {
+  STEXN : a:Type -> wp:wp_t a -> Effect
+  with
+  repr = repr;
+  return = return;
+  bind = bind;
+  stronger = stronger;
+  conjunction = conjunction
+}
+
+inline_for_extraction
+let lift_pure_stexn (a:Type) (wp:pure_wp a{forall p q. (forall x. p x ==> q x) ==> (wp p ==> wp q)}) (f:unit -> PURE a wp)
+: repr a (fun p n -> wp (fun x -> p (Some (x, n))))
+= fun n -> (f (), n)
+
+sub_effect PURE ~> STEXN = lift_pure_stexn
+
+
+effect StExn (a:Type) (pre:nat -> Type0) (post:nat -> option (a & nat) -> Type0) =
+  STEXN a (fun p n -> pre n /\ (forall r. post n r ==> p r))
+
+
+(*** Application ***)
+
+assume val get_n1
+: n:nat ->
+  Pure (option (nat * nat))
+  (requires n > 0)
+  (ensures fun r ->
+    match r with
+    | None -> True
+    | Some (n1, n2) -> n1 == n /\ n2 == n + 1)
+
+type flt = {
+  n1 : nat;
+  n2 : nat;
+  n3 : i:nat{n1 > 0 /\ n2 = n1 + 1 /\ i = n2 + 1}
+}
+
+let get_flt (n:nat)
+: Pure (option flt)
+  (requires n > 0)
+  (ensures fun r ->
+    match r with
+    | None -> True
+    | Some flt -> flt.n1 == n)
+= let r = get_n1 n in
+  match r with
+  | None -> None
+  | Some (x, n) ->
+    let r = get_n1 n in
+    match r with
+    | None -> None
+    | Some (y, n) ->
+      let r = get_n1 n in
+      match r with
+      | None -> None
+      | Some (z, _) -> Some ({ n1 = x; n2 = y; n3 = z })
+
+
+inline_for_extraction
+let get_n1_exn_ (n:nat)
+: unit ->
+  Pure (option (nat * nat))
+  (requires n > 0)
+  (ensures fun r ->
+    match r with
+    | None -> True
+    | Some (n1, n2) -> n1 == n /\ n2 == n + 1)
+= fun _ ->
+  get_n1 n
+
+inline_for_extraction
+let get_n1_exn (n:nat)
+: Exn (nat * nat)
+  (requires n > 0)
+  (ensures fun r ->
+    match r with
+    | None -> True
+    | Some (n1, n2) -> n1 == n /\ n2 == n + 1)
+= EXN?.reflect (get_n1_exn_ n)
+
+inline_for_extraction
+let get_flt_exn (n:nat)
+: Exn flt
+  (requires n > 0)
+  (ensures fun r ->
+    match r with
+    | None -> True
+    | Some flt -> flt.n1 == n)
+= let x, n = get_n1_exn n in
+  let y, n = get_n1_exn n in
+  let z, _ = get_n1_exn n in
+  { n1 = x; n2 = y; n3 = z}
+
+inline_for_extraction
+let get_n1_stexn_ (_:unit)
+: n:nat ->
+  Exn (nat * nat)
+  (requires n > 0)
+  (ensures fun r ->
+    match r with
+    | None -> True
+    | Some (n1, n2) -> n1 == n /\ n2 == n + 1)
+= fun n -> get_n1_exn n
+
+inline_for_extraction
+let get_n1_stexn (_:unit)
+: StExn nat
+  (requires fun n -> n > 0)
+  (ensures fun n r ->
+    match r with
+    | None -> True
+    | Some (n1, n2) -> n1 == n /\ n2 == n + 1)
+= STEXN?.reflect (get_n1_stexn_ ())
+
+let get_n1_stexn2 (_:unit)
+: StExn nat
+  (requires fun n -> n > 0)
+  (ensures fun _ _ -> True)
+= let n = get_n1_stexn () in
+  n
+
+inline_for_extraction
+let get_flt_stexn (_:unit)
+: StExn flt
+  (requires fun n -> n > 0)
+  (ensures fun n r ->
+    match r with
+    | None -> True
+    | Some (flt, _) -> flt.n1 == n)
+= let x = get_n1_stexn () in
+  let y = get_n1_stexn () in
+  let z = get_n1_stexn () in
+  { n1 = x; n2 = y; n3 = z}
+
+
+let get_flt_stexn_reified (n:nat)
+: Pure (option (flt * nat))
+  (requires n > 0)
+  (ensures fun r ->
+    match r with
+    | None -> True
+    | Some (flt, _) -> flt.n1 == n)
+= reify (reify (get_flt_stexn ()) n) ()
